Verify scheduling/scheduler.

theories/scheduling/scheduler.v
@@ -1,9 +1,13 @@
 From zebre Require Import
   prelude.
+From zebre.iris.bi Require Import
+  big_op.
 From zebre.language Require Import
-  notations.
+  notations
+  diaframe.
 From zebre.std Require Import
-  opt.
+  opt
+  for_upto.
 From zebre.saturn Require Import
   spmc_future.
 From zebre.scheduling Require Export
@@ -14,8 +18,10 @@ From zebre.scheduling Require Import
 From zebre Require Import
   options.
 
+Implicit Types v t task : val.
+
 #[local] Notation "'hub'" := (
-  in_type "handle" 0
+in_type "handle" 0
 )(in custom zebre_proj
 ).
 #[local] Notation "'id'" := (
@@ -27,23 +33,30 @@ Section ws_deques.
   Context `{zebre_G : !ZebreG Σ}.
   Context (ws_deques : ws_deques Σ).
 
+  #[local] Definition scheduler_num_round :=
+    2048.
+
+  #[local] Definition scheduler_worker_aux : val :=
+    λ: "hdl",
+      let: "task" := ws_hub_pop ws_deques "hdl".<hub> "hdl".<id> in
+      "task" "hdl".
   #[local] Definition scheduler_worker : val :=
     rec: "scheduler_worker" "hdl" :=
-      let: "task" := ws_hub_pop ws_deques "hdl".<hub> "hdl".<id> in
-      "task" "hdl" ;;
+      scheduler_worker_aux "hdl" ;;
       "scheduler_worker" "hdl".
 
   Definition scheduler_create : val :=
     λ: "sz",
-      let: "t" := ws_hub_create ws_deques (#1 + "sz") in
+      let: "t" := ws_hub_create ws_deques (#1 + "sz") #scheduler_num_round in
       for: "i" := #1 to #1 + "sz" begin
         Fork (scheduler_worker ("t", "i"))
       end ;;
-      "t".
+      ("t", #0).
 
+  #[using="ws_deques"]
   Definition scheduler_run : val :=
-    λ: "t" "task",
-      "task" ("t", #0).
+    λ: "hdl" "task",
+      "task" "hdl".
 
   Definition scheduler_async : val :=
     λ: "hdl" "task",
@@ -59,13 +72,238 @@ Section ws_deques.
       | Some "res" =>
           "res"
       | None =>
-          let: "task" := ws_hub_pop ws_deques "hdl".<hub> "hdl".<id> in
-          "task" "hdl" ;;
+          scheduler_worker_aux "hdl" ;;
           "scheduler_await" "hdl" "fut"
       end.
 End ws_deques.
+
+Class SchedulerG Σ `{zebre_G : !ZebreG Σ} := {
+  #[local] scheduler_G_hub_G :: WsHubG Σ ;
+  #[local] scheduler_G_future_G :: SpmcFutureG Σ ;
+}.
+
+Definition scheduler_Σ := #[
+  ws_hub_Σ ;
+  spmc_future_Σ
+].
+#[global] Instance subG_scheduler_Σ Σ `{zebre_G : !ZebreG Σ} :
+  subG scheduler_Σ Σ →
+  SchedulerG Σ.
+Proof.
+  solve_inG.
+Qed.
+
+Section scheduler_G.
+  Context `{scheduler_G : SchedulerG Σ}.
+  Context (ws_deques : ws_deques Σ).
+
+  #[local] Definition scheduler_inv_inner t : iProp Σ :=
+    ∃ tasks,
+    ws_hub_model ws_deques t tasks ∗
+    [∗ mset] task ∈ tasks,
+      ∀ i,
+      ws_hub_owner ws_deques t (Z.to_nat i) -∗
+      WP task (t, #i)%V {{ _,
+        ws_hub_owner ws_deques t (Z.to_nat i)
+      }}.
+  Definition scheduler_inv t : iProp Σ :=
+    ws_hub_inv ws_deques t (nroot.@"hub") ∗
+    inv (nroot.@"inv") (scheduler_inv_inner t).
+
+  Definition scheduler_handle t hdl : iProp Σ :=
+    ∃ (i : Z),
+    ⌜hdl = (t, #i)%V⌝ ∗
+    ws_hub_owner ws_deques t (Z.to_nat i).
+
+  #[using="ws_deques"]
+  Definition scheduler_future :=
+    spmc_future_inv.
+
+  #[global] Instance scheduler_future_proper t :
+    Proper ((pointwise_relation _ (≡)) ==> (≡)) (scheduler_future t).
+  Proof.
+    solve_proper.
+  Qed.
+
+  #[global] Instance scheduler_handle_timeless t hdl :
+    Timeless (scheduler_handle t hdl).
+  Proof.
+    apply _.
+  Qed.
+  #[global] Instance scheduler_inv_persistent t :
+    Persistent (scheduler_inv t).
+  Proof.
+    apply _.
+  Qed.
+  #[global] Instance scheduler_future_persistent fut Ψ :
+    Persistent (scheduler_future fut Ψ).
+  Proof.
+    apply _.
+  Qed.
+
+  #[local] Lemma scheduler_worker_aux_spec t (i : Z) :
+    {{{
+      scheduler_inv t ∗
+      ws_hub_owner ws_deques t (Z.to_nat i)
+    }}}
+      scheduler_worker_aux ws_deques (t, #i)%V
+    {{{ res,
+      RET res;
+      ws_hub_owner ws_deques t (Z.to_nat i)
+    }}}.
+  Proof.
+    iIntros "%Φ ((#Hhub_inv & #Hinv) & Hhub_owner) HΦ".
+
+    wp_rec.
+
+    awp_smart_apply (ws_hub_pop_spec with "[$Hhub_inv $Hhub_owner]") without "HΦ".
+    iInv "Hinv" as "(%tasks & >Hhub_model & Htasks)".
+    iAaccIntro with "Hhub_model"; first iSteps. iIntros "%task %tasks' (-> & Hhub_model)".
+    iDestruct (big_sepMS_disj_union with "Htasks") as "(Htask & Htasks)".
+    rewrite big_sepMS_singleton.
+    iSplitR "Htask"; first iSteps.
+    iIntros "!> Hhub_owner HΦ". clear.
+
+    wp_smart_apply (wp_wand with "(Htask Hhub_owner) HΦ").
+  Qed.
+  #[local] Lemma scheduler_worker_spec t (i : Z) :
+    {{{
+      scheduler_inv t ∗
+      ws_hub_owner ws_deques t (Z.to_nat i)
+    }}}
+      scheduler_worker ws_deques (t, #i)%V
+    {{{
+      RET (); True
+    }}}.
+  Proof.
+    iIntros "%Φ (#Hinv & Hhub_owner) HΦ".
+
+    iLöb as "HLöb".
+
+    wp_rec.
+    wp_apply (scheduler_worker_aux_spec with "[$Hinv $Hhub_owner]") as (res) "Hhub_owner".
+    wp_smart_apply ("HLöb" with "Hhub_owner HΦ").
+  Qed.
+
+  Lemma scheduler_create_spec sz :
+    (0 ≤ sz)%Z →
+    {{{ True }}}
+      scheduler_create ws_deques #sz
+    {{{ t hdl,
+      RET hdl;
+      scheduler_inv t ∗
+      scheduler_handle t hdl
+    }}}.
+  Proof.
+    iIntros "%Hsz %Φ _ HΦ".
+
+    wp_rec.
+    wp_smart_apply (ws_hub_create_spec with "[//]") as (t) "(#Hhub_inv & Hhub_model & Hhub_owners)"; [lia | done |].
+
+    iMod (inv_alloc _ _ (scheduler_inv_inner t) with "[Hhub_model]") as "#Hinv".
+    { iSteps. rewrite big_sepMS_empty //. }
+
+    rewrite Z.add_1_l Z2Nat.inj_succ // -cons_seq.
+    iDestruct "Hhub_owners" as "(Hhub_owner & Hhub_owners)".
+    wp_smart_apply (for_upto_spec_disentangled' (λ _ _, True)%I with "[Hhub_owners]"); last iSteps.
+    iApply (big_sepL_mono_strong with "Hhub_owners").
+    { rewrite !seq_length. lia. }
+    iIntros "!>" (δ i1 i2 ((-> & Hi1)%lookup_seq & (-> & Hi2)%lookup_seq)) "Hhub_owner %i -> /=".
+    wp_smart_apply (wp_fork with "[Hhub_owner]"); last iSteps. iModIntro.
+    rewrite Z.add_1_l -Nat2Z.inj_succ.
+    wp_smart_apply (scheduler_worker_spec with "[$Hhub_inv $Hinv Hhub_owner]").
+    { rewrite Nat2Z.id //. }
+    iSteps.
+  Qed.
+
+  Lemma scheduler_run_spec Ψ t hdl task :
+    {{{
+      scheduler_inv t ∗
+      scheduler_handle t hdl ∗
+      ( ∀ hdl,
+        scheduler_handle t hdl -∗
+        WP task hdl {{ v,
+          scheduler_handle t hdl ∗
+          Ψ v
+        }}
+      )
+    }}}
+      scheduler_run ws_deques hdl task
+    {{{ v,
+      RET v;
+      scheduler_handle t hdl ∗
+      Ψ v
+    }}}.
+  Proof.
+    iSteps.
+  Qed.
+
+  Lemma scheduler_async_spec Ψ t hdl task :
+    {{{
+      scheduler_inv t ∗
+      scheduler_handle t hdl ∗
+      ( ∀ hdl,
+        scheduler_handle t hdl -∗
+        WP task hdl {{ v,
+          scheduler_handle t hdl ∗
+          □ Ψ v
+        }}
+      )
+    }}}
+      scheduler_async ws_deques hdl task
+    {{{ fut,
+      RET fut;
+      scheduler_handle t hdl ∗
+      scheduler_future fut Ψ
+    }}}.
+  Proof.
+    iIntros "%Φ ((#Hhub_inv & #Hinv) & (%i & -> & Hhub_owner) & Htask) HΦ".
+
+    wp_rec.
+    wp_smart_apply (spmc_future_create_spec with "[//]") as (fut) "(#Hfut_inv & Hfut_producer)".
+
+    awp_smart_apply (ws_hub_push_spec with "[$Hhub_inv $Hhub_owner]") without "HΦ".
+    iInv "Hinv" as "(%tasks & >Hhub_model & Htasks)".
+    iAaccIntro with "Hhub_model". { iFrame. iSteps. } iIntros "Hhub_model".
+    iSplitL.
+    { iExists _. iFrame. rewrite big_sepMS_singleton. iIntros "!> !> %j Hhub_owner".
+      wp_smart_apply (wp_wand with "(Htask [Hhub_owner])") as (v) "((%_j & %Heq & Hhub_owner) & HΨ)"; first iSteps.
+      injection Heq as [= <-].
+      wp_smart_apply (spmc_future_set_spec with "[$Hfut_inv $Hfut_producer $HΨ]").
+      iSteps.
+    }
+    iSteps.
+  Qed.
+
+  Lemma scheduler_await_spec t hdl fut Ψ :
+    {{{
+      scheduler_inv t ∗
+      scheduler_handle t hdl ∗
+      scheduler_future fut Ψ
+    }}}
+      scheduler_await ws_deques hdl fut
+    {{{ v,
+      RET v;
+      scheduler_handle t hdl ∗
+      Ψ v
+    }}}.
+  Proof.
+    iIntros "%Φ ((#Hhub_inv & #Hinv) & (%i & -> & Hhub_owner) & #Hfut_inv) HΦ".
+
+    iLöb as "HLöb".
+
+    wp_rec.
+    wp_smart_apply (spmc_future_try_get_spec with "Hfut_inv") as ([task |]) "HΨ"; first iSteps.
+    wp_smart_apply (scheduler_worker_aux_spec with "[$Hhub_inv $Hinv $Hhub_owner]") as (res) "Hhub_owner".
+    wp_smart_apply ("HLöb" with "Hhub_owner HΦ").
+  Qed.
+End scheduler_G.
 
 #[global] Opaque scheduler_create.
 #[global] Opaque scheduler_run.
 #[global] Opaque scheduler_async.
 #[global] Opaque scheduler_await.
+
+#[global] Opaque scheduler_inv.
+#[global] Opaque scheduler_handle.
+#[global] Opaque scheduler_future.
